simplify rotate functions
faster and no longer 13G of RAM!

Impl.AVL.fst
@@ -275,24 +275,20 @@ let rec insert_avl (#a: Type)
   : Steel (t a) (linked_tree ptr) (fun ptr' -> linked_tree ptr')
   (requires fun h0 ->
     Spec.size_of_tree (v_linked_tree ptr h0) < c /\
+    Spec.height_of_tree (v_linked_tree ptr h0) < c /\
     Spec.is_avl (convert cmp) (v_linked_tree ptr h0))
+
   (ensures fun h0 ptr' h1 ->
     Spec.is_avl (convert cmp) (v_linked_tree ptr h0) /\
     Spec.insert_avl r (convert cmp) (v_linked_tree ptr h0) new_data
-    == v_linked_tree ptr' h1 /\
-    //Spec.is_avl (convert cmp) (v_linked_tree ptr' h1) /\
-    Spec.size_of_tree (v_linked_tree ptr' h1)
-    <= Spec.size_of_tree (v_linked_tree ptr h0) + 1 /\
-    Spec.height_of_tree (v_linked_tree ptr' h1)
-    <= Spec.height_of_tree (v_linked_tree ptr h0) + 1
-  )
+    == v_linked_tree ptr' h1)
   =
-  let h0 = get () in
-  let t1 = hide (v_linked_tree ptr h0) in
-  assert (Spec.size_of_tree (reveal t1) < c);
-  Spec.height_lte_size (v_linked_tree ptr h0);
-  let height_tree = hide (Spec.height_of_tree (reveal t1)) in
-  assert (reveal height_tree < c);
+  //let h0 = get () in
+  //let t1 = hide (v_linked_tree ptr h0) in
+  //assert (Spec.size_of_tree (reveal t1) < c);
+  //Spec.height_lte_size (v_linked_tree ptr h0);
+  //let height_tree = hide (Spec.height_of_tree (reveal t1)) in
+  //assert (reveal height_tree < c);
   //let t2 = hide (Spec.insert_avl
   //  r (convert cmp) (reveal t1) new_data) in
   // TODO: this fails, is this a normalization bug?
@@ -304,13 +300,8 @@ let rec insert_avl (#a: Type)
 
   if is_null_t ptr then (
     (**) null_is_leaf ptr;
-    (**) let second_leaf = create_leaf () in
-    let sr = malloc one in
-    let hr = malloc one in
-    let node = mk_node new_data ptr second_leaf sr hr in
-    let new_tree = malloc node in
-    (**) pack_tree new_tree ptr second_leaf sr hr;
-    return new_tree
+    elim_linked_tree_leaf ptr;
+    create_tree new_data
   ) else (
     (**) let node = unpack_tree ptr in
     let delta = cmp (get_data node) new_data in
@@ -330,55 +321,40 @@ let rec insert_avl (#a: Type)
           (get_size node) (get_height node);
         return ptr
       )
+    ) else if I.gt delta szero then (
+      let h0 = get () in
+      let new_left = insert_avl r cmp (get_left node) new_data in
+      let h1 = get () in
+      assert (v_linked_tree new_left h1
+      == Spec.insert_avl r (convert cmp)
+        (v_linked_tree (get_left node) h0) new_data);
+      Spec.insert_lemma r (convert cmp)
+        (v_linked_tree (get_left node) h0) new_data;
+      assert (Spec.size_of_tree (v_linked_tree new_left h1)
+      <= Spec.size_of_tree (v_linked_tree (get_left node) h0) + 1);
+      assert (Spec.height_of_tree (v_linked_tree new_left h1)
+      <= Spec.height_of_tree (v_linked_tree (get_left node) h0) + 1);
+      let new_ptr = merge_tree_no_alloc
+        (get_data node) new_left (get_right node)
+        (get_size node) (get_height node) ptr in
+      rebalance_avl cmp new_ptr
     ) else (
-      if I.gt delta szero then (
-        let old_left_s = sot_wds (get_left node) in
-        //let old_left_h = hide (hot_wdh (get_left node)) in
-        let new_left = insert_avl r cmp (get_left node) new_data in
-        let new_left_s = sot_wds new_left in
-        let diff = U.sub new_left_s old_left_s in
-        let old_size = read (get_size node) in
-        write (get_size node) (U.add old_size diff);
-        let height_new_left = hot_wdh new_left in
-        let height_right = hot_wdh (get_right node) in
-        //assert (U.v (reveal old_left_h) < reveal height_tree);
-        //assert (U.v (reveal old_left_h) < c - 1);
-        //assert (U.v height_new_left < c);
-        //assert (U.v height_right < reveal height_tree);
-        //assert (U.v height_right < c);
-        let new_height = umax height_new_left height_right in
-        write (get_height node) (U.add new_height one);
-        let new_node = mk_node (get_data node) new_left (get_right node)
-          (get_size node) (get_height node) in
-        write ptr new_node;
-        (**) pack_tree ptr new_left (get_right node)
-          (get_size node) (get_height node);
-        let h = get () in
-        Spec.height_lte_size (v_linked_tree ptr h);
-        Spec.rebalance_height (convert cmp) (v_linked_tree ptr h);
-        rebalance_avl cmp ptr
-      ) else (
-        let old_right_s = sot_wds (get_right node) in
-        let new_right = insert_avl r cmp (get_right node) new_data in
-        let new_right_s = sot_wds new_right in
-        let diff = U.sub new_right_s old_right_s in
-        let old_size = read (get_size node) in
-        write (get_size node) (U.add old_size diff);
-        let height_left = hot_wdh (get_left node) in
-        let height_new_right = hot_wdh new_right in
-        //Spec.height_lte_size (v_linked_tree ptr h0);
-        let new_height = umax height_left height_new_right in
-        write (get_height node) (U.add new_height one);
-        let new_node = mk_node (get_data node) (get_left node) new_right
-          (get_size node) (get_height node) in
-        write ptr new_node;
-        (**) pack_tree ptr (get_left node) new_right
-          (get_size node) (get_height node);
-        let h = get () in
-        Spec.height_lte_size (v_linked_tree ptr h);
-        Spec.rebalance_height (convert cmp) (v_linked_tree ptr h);
-        rebalance_avl cmp ptr
-      )
+      let h0 = get () in
+      let new_right = insert_avl r cmp (get_right node) new_data in
+      let h1 = get () in
+      assert (v_linked_tree new_right h1
+      == Spec.insert_avl r (convert cmp)
+        (v_linked_tree (get_right node) h0) new_data);
+      Spec.insert_lemma r (convert cmp)
+        (v_linked_tree (get_right node) h0) new_data;
+      assert (Spec.size_of_tree (v_linked_tree new_right h1)
+      <= Spec.size_of_tree (v_linked_tree (get_right node) h0) + 1);
+      assert (Spec.height_of_tree (v_linked_tree new_right h1)
+      <= Spec.height_of_tree (v_linked_tree (get_right node) h0) + 1);
+      let new_ptr = merge_tree_no_alloc
+        (get_data node) (get_left node) new_right
+        (get_size node) (get_height node) ptr in
+      rebalance_avl cmp new_ptr
     )
   )
 #pop-options
@@ -546,14 +522,6 @@ let u_of_bool (b:bool) : x:U.t{U.v x = Spec.int_of_bool b}
 //  )
 //#pop-options
 
-let delete_lemma (#a: Type0)
-  (cmp:Spec.cmp a) (t: Spec.avl a cmp) (data_to_rm: a)
-  : Lemma
-  (Spec.height_of_tree (Spec.delete_avl cmp t data_to_rm)
-  <= Spec.height_of_tree t)
-  =
-  Spec.delete_avl_aux_avl cmp t data_to_rm
-
 #push-options "--fuel 1 --ifuel 1 --z3rlimit 100"
 let rec delete_avl (#a: Type0)
   (cmp:cmp a) (ptr: t a) (data_to_rm: a)
@@ -592,16 +560,17 @@ let rec delete_avl (#a: Type0)
     assert (v_linked_tree new_left h1
     == Spec.delete_avl (convert cmp)
       (v_linked_tree (get_left node) h0) data_to_rm);
-    delete_lemma (convert cmp)
+    Spec.delete_lemma (convert cmp)
       (v_linked_tree (get_left node) h0) data_to_rm;
+    assert (Spec.size_of_tree (v_linked_tree new_left h1)
+    <= Spec.size_of_tree (v_linked_tree (get_left node) h0));
     assert (Spec.height_of_tree (v_linked_tree new_left h1)
     <= Spec.height_of_tree (v_linked_tree (get_left node) h0));
     let new_ptr = merge_tree_no_alloc
       (get_data node) new_left (get_right node)
       (get_size node) (get_height node)
       ptr in
-    let new_ptr = rebalance_avl cmp new_ptr in
-    return new_ptr
+    rebalance_avl cmp new_ptr
   ) else (
     let h0 = get () in
     let new_right = delete_avl cmp (get_right node) data_to_rm in
@@ -609,7 +578,27 @@ let rec delete_avl (#a: Type0)
     assert (v_linked_tree new_right h1
     == Spec.delete_avl (convert cmp)
       (v_linked_tree (get_right node) h0) data_to_rm);
-    delete_lemma (convert cmp)
+    Spec.delete_lemma (convert cmp)
+      (v_linked_tree (get_right node) h0) data_to_rm;
+    assert (Spec.size_of_tree (v_linked_tree new_right h1)
+    <= Spec.size_of_tree (v_linked_tree (get_right node) h0));
+    assert (Spec.height_of_tree (v_linked_tree new_right h1)
+    <= Spec.height_of_tree (v_linked_tree (get_right node) h0));
+    let new_ptr = merge_tree_no_alloc
+      (get_data node) (get_left node) new_right
+      (get_size node) (get_height node)
+      ptr in
+    rebalance_avl cmp new_ptr
+  ))
+
+(*)
+    let h0 = get () in
+    let new_right = delete_avl cmp (get_right node) data_to_rm in
+    let h1 = get () in
+    assert (v_linked_tree new_right h1
+    == Spec.delete_avl (convert cmp)
+      (v_linked_tree (get_right node) h0) data_to_rm);
+    Spec.delete_lemma (convert cmp)
       (v_linked_tree (get_right node) h0) data_to_rm;
     assert (Spec.height_of_tree (v_linked_tree new_right h1)
     <= Spec.height_of_tree (v_linked_tree (get_right node) h0));
