Impl.Trees.Rotate.fst
@@ -31,7 +31,7 @@ let rotate_left (#a: Type) (ptr: t a)
   ))
 
   (ensures (fun h0 ptr' h1 ->
-    rotate_left_wdm (v_linked_tree ptr h0)
+    rotate_left (v_linked_tree ptr h0)
     == Some (v_linked_tree ptr' h1)
   ))
   =
@@ -44,30 +44,14 @@ let rotate_left (#a: Type) (ptr: t a)
   (**) node_is_not_null (get_right x_node);
   (**) let z_node = unpack_tree (get_right x_node) in
   let z = get_data z_node in
-  let s1 = sot_wds (get_left x_node) in
-  let s2 = sot_wds (get_left z_node) in
-  let s12 = U.add (U.add s1 s2) one in
 
-  let h1 = hot_wdh (get_left x_node) in
-  let h2 = hot_wdh (get_left z_node) in
-  let h3 = hot_wdh (get_right z_node) in
-  let h12 = if U.gt h1 h2 then U.add h1 one else U.add h2 one in
-  let h123 = if U.gt h12 h3 then U.add h12 one else U.add h3 one in
-  write (get_size z_node) s12;
-  write (get_height z_node) h12;
-  let new_subnode = mk_node x
+  let new_subnode = merge_tree_no_alloc x
     (get_left x_node) (get_left z_node)
-    (get_size z_node) (get_height z_node) in
-  write (get_height x_node) h123;
-  let new_node = mk_node z ptr (get_right z_node)
-    (get_size x_node) (get_height x_node) in
-  write (get_right x_node) new_node;
-  write ptr new_subnode;
-  (**) pack_tree ptr (get_left x_node) (get_left z_node)
-  (get_size z_node) (get_height z_node);
-  (**) pack_tree (get_right x_node) ptr (get_right z_node)
-  (get_size x_node) (get_height x_node);
-  return (get_right x_node)
+    (get_size z_node) (get_height z_node) ptr in
+  let new_node = merge_tree_no_alloc z
+    new_subnode (get_right z_node)
+    (get_size x_node) (get_height x_node) (get_right x_node) in
+  return new_node
 #pop-options
 
 #push-options "--fuel 1 --ifuel 1 --z3rlimit 25"
@@ -82,7 +66,7 @@ let rotate_right (#a: Type) (ptr: t a)
     height_of_tree (opt_get r) <= height_of_tree t
   ))
   (ensures (fun h0 ptr' h1 ->
-    rotate_right_wdm (v_linked_tree ptr h0)
+    rotate_right (v_linked_tree ptr h0)
     == Some (v_linked_tree ptr' h1)
   ))
   =
@@ -95,27 +79,12 @@ let rotate_right (#a: Type) (ptr: t a)
   (**) node_is_not_null (get_left x_node);
   let z_node = unpack_tree (get_left x_node) in
   let z = get_data z_node in
-  let s1 = sot_wds (get_right z_node) in
-  let s2 = sot_wds (get_right x_node) in
-  let s12 = U.add (U.add s1 s2) one in
 
-  let h1 = hot_wdh (get_right z_node) in
-  let h2 = hot_wdh (get_right x_node) in
-  let h3 = hot_wdh (get_left z_node) in
-  let h12 = if U.gt h1 h2 then U.add h1 one else U.add h2 one in
-  let h123 = if U.gt h12 h3 then U.add h12 one else U.add h3 one in
-  write (get_size z_node) s12;
-  write (get_height z_node) h12;
-  let new_subnode = mk_node x (get_right z_node) (get_right x_node)
-    (get_size z_node) (get_height z_node) in
-  write (get_height x_node) h123;
-  let new_node = mk_node z (get_left z_node) ptr
-    (get_size x_node) (get_height x_node) in
-  write (get_left x_node) new_node;
-  write ptr new_subnode;
-  (**) pack_tree ptr (get_right z_node) (get_right x_node)
-    (get_size z_node) (get_height z_node);
-  (**) pack_tree (get_left x_node) (get_left z_node) ptr
-    (get_size x_node) (get_height x_node);
-  return (get_left x_node)
+  let new_subnode = merge_tree_no_alloc x
+    (get_right z_node) (get_right x_node)
+    (get_size z_node) (get_height z_node) ptr in
+  let new_node = merge_tree_no_alloc z
+    (get_left z_node) new_subnode
+    (get_size x_node) (get_height x_node) (get_left x_node) in
+  return new_node
 #pop-options
