Impl.Trees.Rotate2.fst
@@ -1,14 +1,14 @@
 module Impl.Trees.Rotate2
 
-open FStar.Ghost
+//open FStar.Ghost
 
 open Steel.Memory
 open Steel.Effect.Atomic
 open Steel.Effect
 open Steel.Reference
 
-module U = FStar.UInt64
-module I = FStar.Int64
+//module U = FStar.UInt64
+//module I = FStar.Int64
 
 open Spec.Trees
 open Impl.Core
@@ -29,15 +29,10 @@ let rotate_right_left (#a: Type) (ptr: t a)
     height_of_tree (opt_get r) <= height_of_tree t
   ))
   (ensures (fun h0 ptr' h1 ->
-    rotate_right_left_wdm (v_linked_tree ptr h0)
+    rotate_right_left (v_linked_tree ptr h0)
     == Some (v_linked_tree ptr' h1)
   ))
   =
-  let h = get () in
-  assert (size_of_tree (v_linked_tree ptr h) <= c);
-  rotate_right_left_size (v_linked_tree ptr h);
-  assert (size_of_tree (opt_get (rotate_right_left_wdm (v_linked_tree ptr h)))
-  == size_of_tree (v_linked_tree ptr h));
   (**) node_is_not_null ptr;
   // original root node
   (**) let x_node = unpack_tree ptr in
@@ -52,44 +47,15 @@ let rotate_right_left (#a: Type) (ptr: t a)
   // y = get_left (z_node)
   (**) let y_node = unpack_tree (get_left z_node) in
   let y = get_data y_node in
-  let s1 = sot_wds (get_left x_node) in
-  let s2 = sot_wds (get_left y_node) in
-  let s3 = sot_wds (get_right y_node) in
-  let s4 = sot_wds (get_right z_node) in
 
-  let h1 = hot_wdh (get_left x_node) in
-  let h2 = hot_wdh (get_left y_node) in
-  let h3 = hot_wdh (get_right y_node) in
-  let h4 = hot_wdh (get_right z_node) in
-  let h12 = if U.gt h1 h2 then U.add h1 one else U.add h2 one in
-  let h34 = if U.gt h3 h4 then U.add h3 one else U.add h4 one in
-  let h1234 = if U.gt h12 h34 then U.add h12 one else U.add h34 one in
-
-  let s12 = U.add (U.add s1 s2) one in
-  write (get_size y_node) s12;
-  write (get_height y_node) h12;
-  let s34 = U.add (U.add s3 s4) one in
-  write (get_size z_node) s34;
-  write (get_height z_node) h34;
-  write (get_height x_node) h1234;
-
-  let new_x = mk_node x (get_left x_node) (get_left y_node)
-    (get_size y_node) (get_height y_node) in
-  let new_z = mk_node z (get_right y_node) (get_right z_node)
-    (get_size z_node) (get_height z_node) in
-  let new_y = mk_node y ptr (get_right x_node)
-    (get_size x_node) (get_height x_node) in
-
-  write ptr new_x;
-  write (get_right x_node) new_z;
-  write (get_left z_node) new_y;
-
-  (**) pack_tree ptr (get_left x_node) (get_left y_node)
-    (get_size y_node) (get_height y_node);
-  (**) pack_tree (get_right x_node) (get_right y_node) (get_right z_node)
-    (get_size z_node) (get_height z_node);
-  (**) pack_tree (get_left z_node) ptr (get_right x_node)
-    (get_size x_node) (get_height x_node);
-
-  return (get_left z_node)
+  let new_x = merge_tree_no_alloc x
+    (get_left x_node) (get_left y_node)
+    (get_size y_node) (get_height y_node) ptr in
+  let new_z = merge_tree_no_alloc z
+    (get_right y_node) (get_right z_node)
+    (get_size z_node) (get_height z_node) (get_right x_node) in
+  let new_y = merge_tree_no_alloc y
+    new_x new_z
+    (get_size x_node) (get_height x_node) (get_left z_node) in
+  return new_y
 #pop-options
