old/Impl.Trees.Rotate.Old.fst
@@ -1,0 +1,121 @@
+module Impl.Trees.Rotate.Old
+
+open FStar.Ghost
+
+open Steel.Memory
+open Steel.Effect.Atomic
+open Steel.Effect
+open Steel.Reference
+
+module U = FStar.UInt64
+module I = FStar.Int64
+
+open Spec.Trees
+open Impl.Core
+open Impl.Common
+open Impl.Trees
+
+#set-options "--fuel 0 --ifuel 0 --ide_id_info_off"
+
+//@Trees (rotate*)
+#push-options "--fuel 1 --ifuel 1 --z3rlimit 25"
+let rotate_left (#a: Type) (ptr: t a)
+  : Steel (t a)
+  (linked_tree ptr)
+  (fun ptr' -> linked_tree ptr')
+  (requires (fun h0 ->
+    let t = v_linked_tree ptr h0 in
+    let r = rotate_left_wdm t in
+    Some? r /\
+    height_of_tree (opt_get r) <= height_of_tree t
+  ))
+
+  (ensures (fun h0 ptr' h1 ->
+    rotate_left_wdm (v_linked_tree ptr h0)
+    == Some (v_linked_tree ptr' h1)
+  ))
+  =
+  let h = get () in
+  assert (size_of_tree (v_linked_tree ptr h) <= c);
+  rotate_left_size (v_linked_tree ptr h);
+  (**) node_is_not_null ptr;
+  (**) let x_node = unpack_tree ptr in
+  let x = get_data x_node in
+  (**) node_is_not_null (get_right x_node);
+  (**) let z_node = unpack_tree (get_right x_node) in
+  let z = get_data z_node in
+  let s1 = sot_wds (get_left x_node) in
+  let s2 = sot_wds (get_left z_node) in
+  let s12 = U.add (U.add s1 s2) one in
+
+  let h1 = hot_wdh (get_left x_node) in
+  let h2 = hot_wdh (get_left z_node) in
+  let h3 = hot_wdh (get_right z_node) in
+  let h12 = if U.gt h1 h2 then U.add h1 one else U.add h2 one in
+  let h123 = if U.gt h12 h3 then U.add h12 one else U.add h3 one in
+  write (get_size z_node) s12;
+  write (get_height z_node) h12;
+  let new_subnode = mk_node x
+    (get_left x_node) (get_left z_node)
+    (get_size z_node) (get_height z_node) in
+  write (get_height x_node) h123;
+  let new_node = mk_node z ptr (get_right z_node)
+    (get_size x_node) (get_height x_node) in
+  write (get_right x_node) new_node;
+  write ptr new_subnode;
+  (**) pack_tree ptr (get_left x_node) (get_left z_node)
+  (get_size z_node) (get_height z_node);
+  (**) pack_tree (get_right x_node) ptr (get_right z_node)
+  (get_size x_node) (get_height x_node);
+  return (get_right x_node)
+#pop-options
+
+#push-options "--fuel 1 --ifuel 1 --z3rlimit 25"
+let rotate_right (#a: Type) (ptr: t a)
+  : Steel (t a)
+  (linked_tree ptr)
+  (fun ptr' -> linked_tree ptr')
+  (requires (fun h0 ->
+    let t = v_linked_tree ptr h0 in
+    let r = rotate_right_wdm t in
+    Some? r /\
+    height_of_tree (opt_get r) <= height_of_tree t
+  ))
+  (ensures (fun h0 ptr' h1 ->
+    rotate_right_wdm (v_linked_tree ptr h0)
+    == Some (v_linked_tree ptr' h1)
+  ))
+  =
+  let h = get () in
+  assert (size_of_tree (v_linked_tree ptr h) <= c);
+  rotate_right_size (v_linked_tree ptr h);
+  (**) node_is_not_null ptr;
+  (**) let x_node = unpack_tree ptr in
+  let x = get_data x_node in
+  (**) node_is_not_null (get_left x_node);
+  let z_node = unpack_tree (get_left x_node) in
+  let z = get_data z_node in
+  let s1 = sot_wds (get_right z_node) in
+  let s2 = sot_wds (get_right x_node) in
+  let s12 = U.add (U.add s1 s2) one in
+
+  let h1 = hot_wdh (get_right z_node) in
+  let h2 = hot_wdh (get_right x_node) in
+  let h3 = hot_wdh (get_left z_node) in
+  let h12 = if U.gt h1 h2 then U.add h1 one else U.add h2 one in
+  let h123 = if U.gt h12 h3 then U.add h12 one else U.add h3 one in
+  write (get_size z_node) s12;
+  write (get_height z_node) h12;
+  let new_subnode = mk_node x (get_right z_node) (get_right x_node)
+    (get_size z_node) (get_height z_node) in
+  write (get_height x_node) h123;
+  let new_node = mk_node z (get_left z_node) ptr
+    (get_size x_node) (get_height x_node) in
+  write (get_left x_node) new_node;
+  write ptr new_subnode;
+  (**) pack_tree ptr (get_right z_node) (get_right x_node)
+    (get_size z_node) (get_height z_node);
+  (**) pack_tree (get_left x_node) (get_left z_node) ptr
+    (get_size x_node) (get_height x_node);
+  return (get_left x_node)
+#pop-options
